examples/steel/AggregateRefExamples.fst
@@ -60,13 +60,13 @@ let get_y x y
 
 /// Laws relating mk_point to PCM operations
 
-let one_xy : squash (feq (one (prod_pcm point_fields_pcm)) (mk_point None None))
+let one_xy : squash (feq (one point_pcm) (mk_point None None))
 = ()
 
 let merge_xy x y x' y'
-: Lemma (feq (op (prod_pcm point_fields_pcm) (mk_point x y) (mk_point x' y'))
+: Lemma (feq (op point_pcm (mk_point x y) (mk_point x' y'))
              (mk_point (op (point_fields_pcm X) x x') (op (point_fields_pcm Y) y y')))
-  [SMTPat (op (prod_pcm point_fields_pcm) (mk_point x y) (mk_point x' y'))]
+  [SMTPat (op point_pcm (mk_point x y) (mk_point x' y'))]
 = ()
 
 /// Taking pointers to the x and y fields of a point
@@ -77,10 +77,20 @@ let addr_of_x (p: ref 'a point{p.q == point_pcm}) (x y: Ghost.erased (option int
     (fun q ->
        (p `pts_to` mk_point None y) `star`
        (q `pts_to` x))
-= let q = addr_of_lens p int_pcm (field point_fields_pcm X) (mk_point x y) in
+= let q = addr_of_lens p (field point_fields_pcm X) (mk_point x y) in
   A.change_equal_slprop (p `pts_to` _) (p `pts_to` mk_point None y);
   A.change_equal_slprop (q `pts_to` _) (q `pts_to` x);
   A.return q
+
+let un_addr_of_x
+  (p: ref 'a point{p.q == point_pcm})
+  (q: ref 'a (option int){q == ref_focus p int_pcm (field point_fields_pcm X)})
+  (x y: Ghost.erased (option int))
+: SteelT unit
+    ((p `pts_to` mk_point None y) `star` (q `pts_to` x))
+    (fun q -> p `pts_to` mk_point x y)
+= un_addr_of_lens q p (field point_fields_pcm X) (mk_point None y) x;
+  A.change_equal_slprop (p `pts_to` _) (p `pts_to` _)
 
 let addr_of_y (p: ref 'a point{p.q == point_pcm}) (x y: Ghost.erased (option int))
 : SteelT (q:ref 'a (option int){q == ref_focus p int_pcm (field point_fields_pcm Y)})
@@ -88,10 +98,20 @@ let addr_of_y (p: ref 'a point{p.q == point_pcm}) (x y: Ghost.erased (option int
     (fun q ->
        (p `pts_to` mk_point x None) `star`
        (q `pts_to` y))
-= let q = addr_of_lens p int_pcm (field point_fields_pcm Y) (mk_point x y) in
+= let q = addr_of_lens p (field point_fields_pcm Y) (mk_point x y) in
   A.change_equal_slprop (p `pts_to` _) (p `pts_to` mk_point x None);
   A.change_equal_slprop (q `pts_to` _) (q `pts_to` y);
   A.return q
+
+let un_addr_of_y
+  (p: ref 'a point{p.q == point_pcm})
+  (q: ref 'a (option int){q == ref_focus p int_pcm (field point_fields_pcm Y)})
+  (x y: Ghost.erased (option int))
+: SteelT unit
+    ((p `pts_to` mk_point x None) `star` (q `pts_to` y))
+    (fun q -> p `pts_to` mk_point x y)
+= un_addr_of_lens q p (field point_fields_pcm Y) (mk_point x None) y;
+  A.change_equal_slprop (p `pts_to` _) (p `pts_to` _)
 
 /// With the above, we can write the following function that swaps the x and y fields of a given point:
 /// 
@@ -115,27 +135,19 @@ let point_swap (p: ref 'a point{p.q == point_pcm}) (x y: Ghost.erased int)
   let r = addr_of_y p None (Some (Ghost.reveal y)) in
   (* tmp = *q; *)
   let Some tmp = ref_read q (Some (Ghost.reveal x)) in
-  assert (tmp = Ghost.reveal x);
   (* *q = *r; *)
   let Some vy = ref_read r (Some (Ghost.reveal y)) in
-  assert (vy = Ghost.reveal y);
   ref_write q _ vy;
   (* *r = tmp; *)
   ref_write r _ tmp;
   (* Gather *)
+  A.change_equal_slprop (p `pts_to` _) (p `pts_to` _);
   A.change_equal_slprop (q `pts_to` _) (q `pts_to` _);
-  unfocus q p (field point_fields_pcm X) (Some vy);
-  unfocus r p (field point_fields_pcm Y) (Some tmp);
-  A.change_equal_slprop
-    (p `pts_to` put (field point_fields_pcm X) _ _)
-    (p `pts_to` mk_point (Some vy) None);
-  A.change_equal_slprop
-    (p `pts_to` put (field point_fields_pcm Y) _ _)
-    (p `pts_to` mk_point None (Some tmp));
-  gather p (mk_point (Some vy) None) (mk_point None (Some tmp));
-  gather p (mk_point (Ghost.reveal (Ghost.hide None)) None) _;
-  //gather p _ _; // Ask
-  A.change_equal_slprop (p `pts_to` _) _
+  un_addr_of_x p q (Some vy) None;
+  A.change_equal_slprop (p `pts_to` _) (p `pts_to` _);
+  A.change_equal_slprop (r `pts_to` _) (r `pts_to` _);
+  un_addr_of_y p r (Some vy) (Some tmp);
+  A.change_equal_slprop (p `pts_to` _) (p `pts_to` _)
 
 /// Here's a generic swap:
 ///
@@ -189,19 +201,283 @@ let point_swap_generically
   A.change_equal_slprop (r `pts_to` _) (r `pts_to` _);
   generic_swap q r (Ghost.reveal x) (Ghost.reveal y);
   (* Gather *)
+  A.change_equal_slprop (p `pts_to` _) (p `pts_to` _);
   A.change_equal_slprop (q `pts_to` _) (q `pts_to` _);
+  un_addr_of_x p q (Some (Ghost.reveal y)) None;
+  A.change_equal_slprop (p `pts_to` _) (p `pts_to` _);
   A.change_equal_slprop (r `pts_to` _) (r `pts_to` _);
-  unfocus q p (field point_fields_pcm X) (Some (Ghost.reveal y));
-  unfocus r p (field point_fields_pcm Y) (Some (Ghost.reveal x));
+  un_addr_of_y p r (Some (Ghost.reveal y)) (Some (Ghost.reveal x));
+  A.change_equal_slprop (p `pts_to` _) (p `pts_to` _)
+
+/// Example 2: pointers to nested fields
+///
+/// Here's a struct representing a line segment by its two endpoints:
+///   struct line { struct point p1; struct point p2; };
+///
+/// Carrier of PCM for line:
+
+type line_field = | P1 | P2
+let line_fields k = match k with
+  | P1 -> point
+  | P2 -> point
+let line = restricted_t line_field line_fields
+
+/// PCM for line:
+
+let line_fields_pcm k : pcm (line_fields k) = match k with
+  | P1 -> point_pcm
+  | P2 -> point_pcm
+let line_pcm = prod_pcm line_fields_pcm
+
+/// (mk_line p1 p2) represents (struct line){.p1 = p1, .p2 = p2}
+
+let mk_line_f (p1 p2: point) (k: line_field): line_fields k = match k with
+  | P1 -> p1
+  | P2 -> p2
+let mk_line (p1 p2: point): line = on_domain line_field (mk_line_f p1 p2)
+
+/// Laws about putting/getting the x and y fields of a (mk_line x y)
+
+let put_p1 p1' p1 p2
+: Lemma (feq (put (field line_fields_pcm P1) p1' (mk_line p1 p2)) (mk_line p1' p2))
+  [SMTPat (put (field line_fields_pcm P1) p1' (mk_line p1 p2))]
+= ()
+
+let get_p1 p1 p2
+: Lemma (get (field line_fields_pcm P1) (mk_line p1 p2) == p1)
+  [SMTPat (get (field line_fields_pcm P1) (mk_line p1 p2))]
+= ()
+
+let put_p2 p2' p1 p2
+: Lemma (feq (put (field line_fields_pcm P2) p2' (mk_line p1 p2)) (mk_line p1 p2'))
+  [SMTPat (put (field line_fields_pcm P2) p2' (mk_line p1 p2))]
+= ()
+
+let get_p2 p1 p2
+: Lemma (get (field line_fields_pcm P2) (mk_line p1 p2) == p2)
+  [SMTPat (get (field line_fields_pcm P2) (mk_line p1 p2))]
+= ()
+
+/// Laws relating mk_line to PCM operations
+
+let one_line : squash (feq (one line_pcm) (mk_line (one point_pcm) (one point_pcm)))
+= ()
+
+let merge_line p1 p2 p1' p2'
+: Lemma (feq (op line_pcm (mk_line p1 p2) (mk_line p1' p2'))
+             (mk_line (op (line_fields_pcm P1) p1 p1') (op (line_fields_pcm P2) p2 p2')))
+  [SMTPat (op line_pcm (mk_line p1 p2) (mk_line p1' p2'))]
+= ()
+
+/// Taking pointers to the p1 and p2 fields of a line
+
+let addr_of_p1 (p: ref 'a line{p.q == line_pcm}) (p1 p2: Ghost.erased point)
+: SteelT (q:ref 'a point{q == ref_focus p point_pcm (field line_fields_pcm P1)})
+    (p `pts_to` mk_line p1 p2)
+    (fun q ->
+       (p `pts_to` mk_line (one point_pcm) p2) `star`
+       (q `pts_to` p1))
+= let q = addr_of_lens p (field line_fields_pcm P1) (mk_line p1 p2) in
+  A.change_equal_slprop (p `pts_to` _) (p `pts_to` mk_line (one point_pcm) p2);
+  A.change_equal_slprop (q `pts_to` _) (q `pts_to` p1);
+  A.return q
+
+let un_addr_of_p1
+  (p: ref 'a line{p.q == line_pcm})
+  (q: ref 'a point{q == ref_focus p point_pcm (field line_fields_pcm P1)})
+  (p1 p2: Ghost.erased point)
+: SteelT unit
+    ((p `pts_to` mk_line (one point_pcm) p2) `star` (q `pts_to` p1))
+    (fun q -> p `pts_to` mk_line p1 p2)
+= un_addr_of_lens q p (field line_fields_pcm P1) (mk_line (one point_pcm) p2) p1;
+  A.change_equal_slprop (p `pts_to` _) (p `pts_to` _)
+
+let addr_of_p2 (p: ref 'a line{p.q == line_pcm}) (p1 p2: Ghost.erased point)
+: SteelT (q:ref 'a point{q == ref_focus p point_pcm (field line_fields_pcm P2)})
+    (p `pts_to` mk_line p1 p2)
+    (fun q ->
+       (p `pts_to` mk_line p1 (one point_pcm)) `star`
+       (q `pts_to` p2))
+= let q = addr_of_lens p (field line_fields_pcm P2) (mk_line p1 p2) in
+  A.change_equal_slprop (p `pts_to` _) (p `pts_to` mk_line p1 (one point_pcm));
+  A.change_equal_slprop (q `pts_to` _) (q `pts_to` p2);
+  A.return q
+
+let un_addr_of_p2
+  (p: ref 'a line{p.q == line_pcm})
+  (q: ref 'a point{q == ref_focus p point_pcm (field line_fields_pcm P2)})
+  (p1 p2: Ghost.erased point)
+: SteelT unit
+    ((p `pts_to` mk_line p1 (one point_pcm)) `star` (q `pts_to` p2))
+    (fun q -> p `pts_to` mk_line p1 p2)
+= un_addr_of_lens q p (field line_fields_pcm P2) (mk_line p1 (one point_pcm)) p2;
+  A.change_equal_slprop (p `pts_to` _) (p `pts_to` _)
+
+/// Reflect a line segment across the line y=x and reverse its direction
+///
+/// void reflect_and_reverse(struct line *p) {
+///   generic_swap(&p.p1.x, &p.p2.y);
+///   generic_swap(&p.p1.y, &p.p2.x);
+/// }
+
+#push-options "--z3rlimit 20"
+let reflect_and_reverse
+  (p: ref 'a line{p.q == line_pcm}) (x1 y1 x2 y2: Ghost.erased int)
+: SteelT unit
+    (p `pts_to`
+      mk_line
+        (mk_point (Some (Ghost.reveal x1)) (Some (Ghost.reveal y1)))
+        (mk_point (Some (Ghost.reveal x2)) (Some (Ghost.reveal y2))))
+    (fun _ ->
+      p `pts_to`
+        mk_line
+          (mk_point (Some (Ghost.reveal y2)) (Some (Ghost.reveal x2)))
+          (mk_point (Some (Ghost.reveal y1)) (Some (Ghost.reveal x1))))
+= (* Take all the requisite pointers *)
+  A.change_equal_slprop (p `pts_to` _) (p `pts_to` _);
+  let pp1 =
+    addr_of_p1 p
+      (mk_point (Some (Ghost.reveal x1)) (Some (Ghost.reveal y1)))
+      (mk_point (Some (Ghost.reveal x2)) (Some (Ghost.reveal y2)))
+  in
+  A.change_equal_slprop (p `pts_to` _) (p `pts_to` _);
+  let pp2 =
+    addr_of_p2 p
+      (one point_pcm)
+      (mk_point (Some (Ghost.reveal x2)) (Some (Ghost.reveal y2)))
+  in
+  (* &p.p1.x *)
+  A.change_equal_slprop (pp1 `pts_to` _) (pp1 `pts_to` _);
+  let pp1x = addr_of_x pp1 (Some (Ghost.reveal x1)) (Some (Ghost.reveal y1)) in
+  (* &p.p1.y *)
+  A.change_equal_slprop (pp1 `pts_to` _) (pp1 `pts_to` _);
+  let pp1y = addr_of_y pp1 None (Some (Ghost.reveal y1)) in
+  (* &p.p2.x *)
+  A.change_equal_slprop (pp2 `pts_to` _) (pp2 `pts_to` _);
+  let pp2x = addr_of_x pp2 (Some (Ghost.reveal x2)) (Some (Ghost.reveal y2)) in
+  (* &p.p2.y *)
+  A.change_equal_slprop (pp2 `pts_to` _) (pp2 `pts_to` _);
+  let pp2y = addr_of_y pp2 None (Some (Ghost.reveal y2)) in
+  (* generic_swap(&p.p1.x, &p.p2.y); *)
+  generic_swap pp1x pp2y x1 y2;
+  (* generic_swap(&p.p1.y, &p.p2.x); *)
+  generic_swap pp1y pp2x y1 x2;
+  (* Gather p1 *)
+  A.change_equal_slprop (pp1x `pts_to` _) (pp1x `pts_to` _);
+  A.change_equal_slprop (pp1 `pts_to` _) (pp1 `pts_to` _);
+  un_addr_of_x pp1 pp1x (Some (Ghost.reveal y2)) None;
+  A.change_equal_slprop (pp1y `pts_to` _) (pp1y `pts_to` _);
+  A.change_equal_slprop (pp1 `pts_to` _) (pp1 `pts_to` _);
+  un_addr_of_y pp1 pp1y (Some (Ghost.reveal y2)) (Some (Ghost.reveal x2));
+  (* Gather p2 *)
+  A.change_equal_slprop (pp2x `pts_to` _) (pp2x `pts_to` _);
+  A.change_equal_slprop (pp2 `pts_to` _) (pp2 `pts_to` _);
+  un_addr_of_x pp2 pp2x (Some (Ghost.reveal y1)) None;
+  A.change_equal_slprop (pp2y `pts_to` _) (pp2y `pts_to` _);
+  A.change_equal_slprop (pp2 `pts_to` _) (pp2 `pts_to` _);
+  un_addr_of_y pp2 pp2y (Some (Ghost.reveal y1)) (Some (Ghost.reveal x1));
+  (* Gather p *)
+  A.change_equal_slprop (pp1 `pts_to` _) (pp1 `pts_to` _);
+  A.change_equal_slprop (p `pts_to` _) (p `pts_to` _);
+  un_addr_of_p1 p pp1 (mk_point (Some (Ghost.reveal y2)) (Some (Ghost.reveal x2))) (one point_pcm);
+  A.change_equal_slprop (pp2 `pts_to` _) (pp2 `pts_to` _);
+  A.change_equal_slprop (p `pts_to` _) (p `pts_to` _);
+  un_addr_of_p2 p pp2
+    (mk_point (Some (Ghost.reveal y2)) (Some (Ghost.reveal x2)))
+    (mk_point (Some (Ghost.reveal y1)) (Some (Ghost.reveal x1)));
+  A.change_equal_slprop (p `pts_to` _) (p `pts_to` _)
+#pop-options
+
+(*
+addr_of
+  (r `pts_to` xs)
+  (r `pts_to` xs \ k `star` s `pts_to` xs k)
+  
+addr_of
+  (r `pts_to` xs `star` s `pts_to` y)
+  (r `pts_to` xs [k `mapsto` y])
+  *)
+
+(*
+
+  A.change_equal_slprop (pp1x `pts_to` _) (pp1x `pts_to` _);
+  A.change_equal_slprop (pp1y `pts_to` _) (pp1y `pts_to` _);
+  unfocus pp1x pp1 (field point_fields_pcm X) (Some (Ghost.reveal y2));
+  unfocus pp1y pp1 (field point_fields_pcm Y) (Some (Ghost.reveal x2));
   A.change_equal_slprop
-    (p `pts_to` put (field point_fields_pcm X) _ _)
-    (p `pts_to` mk_point (Some (Ghost.reveal y)) None);
+    (pp1 `pts_to` put (field point_fields_pcm X) _ _)
+    (pp1 `pts_to` mk_point (Some (Ghost.reveal y2)) None);
   A.change_equal_slprop
-    (p `pts_to` put (field point_fields_pcm Y) _ _)
-    (p `pts_to` mk_point None (Some (Ghost.reveal x)));
-  gather p (mk_point (Some (Ghost.reveal y)) None) (mk_point None (Some (Ghost.reveal x)));
-  gather p (mk_point (Ghost.reveal (Ghost.hide None)) None) _;
-  A.change_equal_slprop (p `pts_to` _) _
+    (pp1 `pts_to` put (field point_fields_pcm Y) _ _)
+    (pp1 `pts_to` mk_point None (Some (Ghost.reveal x2)));
+  gather pp1 (mk_point (Some (Ghost.reveal y2)) None) (mk_point None (Some (Ghost.reveal x2)));
+  gather pp1 (mk_point (Ghost.reveal (Ghost.hide None)) None) _;
+  (* Gather p2 *)
+  A.change_equal_slprop (pp2x `pts_to` _) (pp2x `pts_to` _);
+  A.change_equal_slprop (pp2y `pts_to` _) (pp2y `pts_to` _);
+  unfocus pp2x pp2 (field point_fields_pcm X) (Some (Ghost.reveal y1));
+  unfocus pp2y pp2 (field point_fields_pcm Y) (Some (Ghost.reveal x1));
+  A.change_equal_slprop
+    (pp2 `pts_to` put (field point_fields_pcm X) _ _)
+    (pp2 `pts_to` mk_point (Some (Ghost.reveal y1)) None);
+  A.change_equal_slprop
+    (pp2 `pts_to` put (field point_fields_pcm Y) _ _)
+    (pp2 `pts_to` mk_point None (Some (Ghost.reveal x1)));
+  gather pp2 (mk_point (Some (Ghost.reveal y1)) None) (mk_point None (Some (Ghost.reveal x1)));
+  gather pp2 (mk_point (Ghost.reveal (Ghost.hide None)) None) _;
+  (* Gather p *)
+  A.change_equal_slprop (pp1 `pts_to` _) (pp1 `pts_to` _);
+  A.change_equal_slprop (pp2 `pts_to` _) (pp2 `pts_to` _);
+  unfocus pp1 p (field line_fields_pcm P1)
+    (mk_point (Some (Ghost.reveal y2)) (Some (Ghost.reveal x2)));
+  unfocus pp2 p (field line_fields_pcm P2)
+    (mk_point (Some (Ghost.reveal y1)) (Some (Ghost.reveal x1)));
+  A.change_equal_slprop
+    (p `pts_to` put (field line_fields_pcm P1) _ _)
+    (p `pts_to`
+      mk_line
+        (mk_point (Some (Ghost.reveal y2)) (Some (Ghost.reveal x2)))
+        (one point_pcm));
+  A.change_equal_slprop
+    (p `pts_to` put (field line_fields_pcm P2) _ _)
+    (p `pts_to`
+      mk_line
+        (one point_pcm)
+        (mk_point (Some (Ghost.reveal y1)) (Some (Ghost.reveal x1))));
+  gather p
+    (mk_line
+      (mk_point (Some (Ghost.reveal y2)) (Some (Ghost.reveal x2)))
+      (one point_pcm))
+    (mk_line
+       (one point_pcm)
+       (mk_point (Some (Ghost.reveal y1)) (Some (Ghost.reveal x1))));
+  gather p (mk_line (Ghost.reveal (Ghost.hide (one point_pcm))) (one point_pcm)) _;
+  //A.change_equal_slprop (pp2 `pts_to` _) _;
+  (* int *r = &p.p1.y; *)
+  (* int *s = &p.p2.x; *)
+  (* int *t = &p.p2.y; *)
+  A.sladmit();
+  A.return ()
+#pop-options
+*)
+
+(*
+pts_to r x
+(fun r' -> pts_to r' x')
+(requires (fun _ -> x is in case A))
+(ensures (fun _ r' _ -> x == A x'))
+A x' = (|TagA, x'|)
+
+(q:ref .) (t: erased tag)
+pts_to q (t, u)
+(requires (fun _ -> u is in case (tag_denote t)))
+
+(q:ref .) (t: erased tag)
+(r:ref . = the union inside q)
+pts_to q (t, one) `star` pts_to r x
+
+(requires (fun _ -> x is in case (tag_denote t)))
+*)
 
 (*
 to print proof state, try:
